[statelib crdt examples] gos - progress.

ml_sources/examples/crdt/statelib/examples/grow_only_set/grow_only_set_code.ml
@@ -14,11 +14,6 @@ let mutator : ('a, 'stTy) mutatorFnTy =
 let set_union (s1 : 'a aset) (s2 : 'a aset) : 'a aset =
   set_foldl (fun su e -> set_add e su) s1 s2
 
-(* TODO: move to the aneris lib. *)
-let set_serializer (elt_ser[@metavar "serializer"] : 'a serializer) : 'a aset serializer =
-  list_serializer elt_ser
-
-
 let merge (st1 : 'a stTy) (st2 : 'a stTy) : 'a stTy =
   set_union st1 st2
 
@@ -28,12 +23,9 @@ let init_st () = set_empty ()
 
 let gos_crdt : ('a, 'a stTy) crdtTy = fun () -> ((init_st, mutator), merge)
 
-let st_ser (elt_ser[@metavar "serializer"] : 'a serializer) : 'a alist serializer =
-  set_serializer elt_ser
-
-let gos_init (elt_ser[@metavar "serializer"] : 'a serializer) (addrs : saddr alist) (rid : int) =
+let gos_init  (elt_ser[@metavar "val"])(elt_deser[@metavar "val"])
+    (addrs : saddr alist) (rid : int) =
   let initRes =
-    statelib_init (st_ser elt_ser).s_ser (st_ser elt_ser).s_deser addrs rid gos_crdt in
+    statelib_init (list_ser elt_ser) (list_deser elt_deser) addrs rid gos_crdt in
   let (get_state, update) = initRes in
-  let eval st = eval_state (get_state st) in
-  (eval, update)
+  (get_state, update)
